LocallyNameless/STLCv2.v
@@ -1,0 +1,854 @@
+Require Import
+  List
+  Coq.Classes.DecidableClass.
+
+Import ListNotations.
+
+From FormalSystems Require Export LocallyNameless.LocallyNameless.
+
+Inductive Ty : Type :=
+| TyUnit : Ty
+| TyFun  : Ty -> Ty -> Ty.
+
+Fixpoint eq_dec_Ty (A B : Ty) : bool :=
+match A, B with
+| TyUnit, TyUnit => true
+| TyFun A1 A2, TyFun B1 B2 => andb (eq_dec_Ty A1 B1) (eq_dec_Ty A2 B2)
+| _, _ => false
+end.
+
+#[export, refine] Instance Decidable_eq_Ty :
+  forall A B : Ty, Decidable (A = B) :=
+{
+  Decidable_witness := eq_dec_Ty A B;
+}.
+Proof.
+  revert B.
+  induction A as [| A1 IH1 A2 IH2]; cbn; intros [| B1 B2];
+    only 1-3: now firstorder congruence.
+  split.
+  - intros [H1 H2]%andb_prop.
+    now f_equal; [apply IH1 | apply IH2].
+  - intros [= -> ->].
+    apply andb_true_intro.
+    now rewrite IH1, IH2.
+Defined.
+
+Inductive Tm : Type :=
+| fvar (a : Atom) : Tm
+| bvar : nat -> Tm
+| abs  : Tm -> Tm
+| app  : Tm -> Tm -> Tm.
+
+Coercion fvar : Atom >-> Tm.
+Coercion bvar : nat >-> Tm.
+
+Fixpoint subst (x : Atom) (u t : Tm) : Tm :=
+match t with
+| fvar y    => if decide (x = y) then u else fvar y
+| bvar n    => bvar n
+| abs t'    => abs (subst x u t')
+| app t1 t2 => app (subst x u t1) (subst x u t2)
+end.
+
+Notation "t [[ x := u ]]" := (subst x u t) (at level 68).
+
+Fixpoint fv (t : Tm) : list Atom :=
+match t with
+| fvar x    => [x]
+| bvar _    => []
+| abs t'    => fv t'
+| app t1 t2 => fv t1 ++ fv t2
+end.
+
+Lemma subst_fresh :
+  forall (x : Atom) (u t : Tm),
+    x # fv t -> t [[ x := u ]] = t.
+Proof.
+  induction t; cbn; intros.
+  - decide (x = a); [| easy].
+    now firstorder congruence.
+  - easy.
+  - now rewrite IHt.
+  - red in H; rewrite in_app_iff in H.
+    now firstorder congruence.
+Qed.
+
+Fixpoint open' (t : Tm) (i : nat) (u : Tm) : Tm :=
+match t with
+| fvar a    => fvar a
+| bvar j    => if decide (i = j) then u else bvar j
+| abs t'    => abs (open' t' (S i) u)
+| app t1 t2 => app (open' t1 i u) (open' t2 i u)
+end.
+
+(* Notation "t {{ i ~> u }}" := (open' t i u) (at level 68). *)
+
+Fixpoint close' (t : Tm) (i : nat) (a : Atom) : Tm :=
+match t with
+| fvar x    => if decide (a = x) then bvar i else fvar x
+| bvar n    => bvar n
+| abs t'    => abs (close' t' (S i) a)
+| app t1 t2 => app (close' t1 i a) (close' t2 i a)
+end.
+
+(* Notation "t {{ i <~ a }}" := (close' t i a) (at level 68). *)
+
+(*
+#[export] Instance Open_Tm : Open nat Atom Tm :=
+  fix open (t : Tm) (i : nat) (u : Tm) : Tm :=
+    let _ : Open _ _ _ := @open in
+    match t with
+    | fvar a    => fvar a
+    | bvar j    => if decide (i = j) then u else bvar j
+    | abs t'    => abs (t' {{ S i ~> u }})
+    | app t1 t2 => app (t1 {{ i ~> u }}) (t2 {{ i ~> u }})
+    end.
+
+#[export] Instance Close_Tm : Close nat Atom Tm :=
+  fix close (t : Tm) (i : nat) (a : Atom) : Tm :=
+    let _ : Close _ _ _ := @close in
+    match t with
+    | fvar x    => if decide (a = x) then bvar i else fvar x
+    | bvar n    => bvar n
+    | abs t'    => abs (t' {{ S i <~ a }})
+    | app t1 t2 => app (t1 {{ i <~ a }}) (t2 {{ i <~ a }})
+    end.
+*)
+
+#[export] Instance Open_Tm : Open nat Atom Tm :=
+  fix open (t : Tm) (i : nat) (a : Atom) : Tm :=
+    match t with
+    | fvar a    => fvar a
+    | bvar j    => if decide (i = j) then a else bvar j
+    | abs t'    => abs (open t' (S i) a)
+    | app t1 t2 => app (open t1 i a) (open t2 i a)
+    end.
+
+#[export] Instance Close_Tm : Close nat Atom Tm :=
+  fix close (t : Tm) (i : nat) (a : Atom) : Tm :=
+    match t with
+    | fvar x    => if decide (a = x) then bvar i else fvar x
+    | bvar n    => bvar n
+    | abs t'    => abs (close t' (S i) a)
+    | app t1 t2 => app (close t1 i a) (close t2 i a)
+    end.
+
+(*
+#[export] Instance Open_Tm : Open nat Atom Tm := open'.
+#[export] Instance Close_Tm : Close nat Atom Tm := close'.
+*)
+
+(*
+Lemma open_from_subst :
+  forall (t : Tm) (i : nat) (x : Atom) (u : Tm),
+    x # fv t ->
+      t {{ i ~> u }} = t {{ i ~> x }} [[ x := u ]].
+Proof.
+  induction t; cbn; intros.
+  - now decide (x = a); subst; firstorder.
+  - now decide_all.
+  - now rewrite <- IHt.
+  - red in H; rewrite in_app_iff in H.
+    now rewrite <- IHt1, <- IHt2; firstorder.
+Qed.
+*)
+
+#[export, refine] Instance LocallyNameless_Tm :
+  LocallyNameless nat Atom Tm Open_Tm Close_Tm := {}.
+Proof.
+  all: induction t; cbn; intros;
+    [now decide_all | now decide_all | now rewrite IHt; try congruence | now rewrite IHt1, IHt2].
+Defined.
+
+Definition Fresh' (x : Atom) (t : Tm) : Prop :=
+  t {{ 0 <~ x }} = t.
+
+(* Lemma 2.4 from the paper *)
+Lemma Fresh'_invariant_aux :
+  forall (x : Atom) (t : Tm) (i j : nat),
+    t {{ j <~ x }} = t <-> t {{ i <~ x }} = t.
+Proof.
+  now split; intros [= <-]; rewrite close_close_eq.
+Qed.
+
+Lemma Fresh'_invariant_aux' :
+  forall (x : Atom) (t : Tm) (i : nat),
+    t {{ i <~ x }} = t <-> forall j : nat, t {{ j <~ x }} = t.
+Proof.
+  split; [| easy].
+  now intros [= <-] j; rewrite close_close_eq.
+Qed.
+
+Lemma Fresh'_invariant :
+  forall (x : Atom) (t : Tm) (i : nat),
+    Fresh' x t <-> t {{ i <~ x }} = t.
+Proof.
+  intros; unfold Fresh'.
+  now apply Fresh'_invariant_aux.
+Qed.
+
+Lemma Fresh'_spec :
+  forall (x : Atom) (t : Tm),
+    Fresh' x t <-> x # fv t.
+Proof.
+  split; unfold Fresh, Fresh'.
+  - intros H.
+    induction t; cbn; intros.
+    + intros [-> |]; [| easy].
+      cbn in H.
+      now decide (x = x).
+    + easy.
+    + apply IHt.
+      cbn in H; inversion H; subst.
+      now rewrite close_close_eq.
+    + cbn in H; inversion H; subst.
+      rewrite H1, H2, in_app_iff.
+      now firstorder.
+  - induction t; cbn.
+    + now decide_all; firstorder.
+    + easy.
+    + intros Hfresh.
+      now rewrite <- IHt, close_close_eq by easy.
+    + rewrite in_app_iff.
+      now firstorder congruence.
+Qed.
+
+Definition opensubst t i u :=
+  t {{ i ~> fresh (fv t) }} [[ fresh (fv t) := u ]].
+
+Notation "t {[ i ~> u ]}" := (opensubst t i u) (at level 68).
+
+(*
+Lemma open_open :
+  forall (t : Tm) (i j : nat) (u1 u2 : Tm),
+    i <> j ->
+    t {[ i ~> u1 ]} {[ j ~> u2 ]} = t {[ i ~> u1 ]} ->
+      t {[ j ~> u2 ]} = t.
+Proof.
+  induction t; cbn; intros * Hneq H.
+  - easy.
+  - decide (i = n); subst; cbn; [| easy].
+    decide (j = n); [| easy].
+    now congruence.
+  - inversion H.
+    f_equal.
+    eapply IHt, H1.
+    now congruence.
+  - inversion H.
+    f_equal.
+    + now eapply IHt1, H1.
+    + now eapply IHt2, H2.
+Qed.
+*)
+
+Inductive lc : Tm -> Prop :=
+| lc_fvar :
+  forall x : Atom,
+    lc x
+| lc_abs :
+  forall (t : Tm) (l : list Atom)
+    (Hcof : forall x, x # l -> lc (t {{ 0 ~> x }})),
+    lc (abs t)
+| lc_app :
+  forall t1 t2 : Tm,
+    lc t1 ->
+    lc t2 ->
+    lc (app t1 t2).
+
+#[export] Hint Constructors lc : core.
+
+Definition lci (i : nat) (t : Tm) : Prop :=
+  forall j : nat, i <= j -> t {{ j ~> fresh (fv t) }} = t.
+
+Lemma lci_spec :
+  forall t : Tm,
+    lc t -> lci 0 t.
+Proof.
+  unfold lci.
+  induction 1; intros j Hle.
+  - now cbn.
+  - cbn; f_equal.
+    specialize (Hcof (fresh l) (fresh_spec l)).
+    inversion Hcof; subst.
+Abort.
+
+(*
+Definition lci (i : nat) (t : Tm) : Prop :=
+  forall j : nat, i <= j -> exists a : Atom, t {{ j ~> a }} = t.
+
+Lemma lci_spec :
+  forall t : Tm,
+    lc t -> lci 0 t.
+Proof.
+  unfold lci.
+  induction 1; intros j Hle.
+  - now exists x.
+  - destruct (H (fresh l) (fresh_spec l) j Hle) as [a Heq].
+    exists a; cbn; f_equal.
+    admit.
+  - 
+*)
+
+(*
+Lemma open_lc :
+  forall (t : Tm) (i : nat) (u : Tm),
+    lc t -> t {{ i ~> u }} = t.
+Proof.
+  intros t i u Hlc; revert i u.
+  induction Hlc; cbn; intros; [easy | | now congruence].
+  f_equal.
+  eapply open_open with (i := 0); [easy |].
+  apply (H (fresh l)).
+  now solve_fresh.
+Qed.
+
+Lemma subst_open :
+  forall (t : Tm) (i : nat) (u1 : Tm) (x : Atom) (u2 : Tm),
+    lc u2 ->
+    t {{ i ~> u1 }} [[ x := u2 ]]
+      =
+    t [[ x := u2 ]] {{ i ~> u1 [[ x := u2 ]] }}.
+Proof.
+  induction t; cbn; intros.
+  - rewrite open_lc; [easy |].
+    now decide (x = a).
+  - now decide (i = n).
+  - now rewrite IHt.
+  - now rewrite IHt1, IHt2.
+Qed.
+*)
+
+Lemma open_open :
+  forall (t : Tm) (i j : nat) (a b : Atom),
+    i <> j ->
+    t {{ i ~> a }} {{ j ~> b }} = t {{ i ~> a }} ->
+      t {{ j ~> b }} = t.
+Proof.
+  induction t; cbn; intros * Hneq H.
+  - easy.
+  - now revert H; decide_all.
+  - f_equal.
+    eapply IHt; cycle 1; unfold opensubst; cbn.
+    + inversion H; cbn in *.
+      now apply H1.
+    + now congruence.
+  - inversion H.
+    f_equal.
+    + now apply IHt1 in H1.
+    + now apply IHt2 in H2.
+Qed.
+
+Lemma open_lc :
+  forall (t : Tm) (i : nat) (a : Atom),
+    lc t -> t {{ i ~> a }} = t.
+Proof.
+  intros t i a Hlc; revert i a.
+  induction Hlc; cbn; intros; [easy | | now congruence].
+  f_equal.
+  eapply open_open with (i := 0); [easy |].
+  apply (H (fresh l)).
+  now solve_fresh.
+Qed.
+
+Lemma subst_open :
+  forall (t : Tm) (i : nat) (a b x : Atom),
+    t {{ i ~> a }} [[ x := b ]]
+      =
+    t [[ x := b ]] {{ i ~> if decide (a = x) then b else a }}.
+Proof.
+  induction t; cbn; intros.
+  - now decide_all.
+  - now decide_all.
+  - now rewrite IHt.
+  - now rewrite IHt1, IHt2.
+Qed.
+
+Lemma open_subst :
+  forall (t : Tm) (a b : Atom) (u : Tm),
+    a <> b -> lc u ->
+    t [[ a := u ]] {{ 0 ~> b }} = t {{ 0 ~> b }} [[ a := u ]].
+Proof.
+  induction t; cbn; intros.
+  - decide_all.
+    inversion H0; subst; cbn.
+    + easy.
+    + admit.
+    +
+    now decide (x = a).
+  - now decide (i = n).
+  - now rewrite IHt.
+  - now rewrite IHt1, IHt2.
+Restart.
+Qed.
+
+Lemma lc_subst :
+  forall (t : Tm) (x : Atom) (u : Tm),
+    lc t -> lc u -> lc (t [[ x := u ]]).
+Proof.
+  intros t x u Ht Hu; revert x u Hu.
+  induction Ht; cbn; intros.
+  - now decide (x0 = x).
+  - apply lc_abs with (x :: l).
+    intros y Hin.
+    rewrite open_subst; [| now firstorder | easy].
+    apply H; [| easy].
+    now firstorder.
+  - now constructor; [apply IHHt1 | apply IHHt2].
+Qed.
+
+Definition Ctx : Type := list (Atom * Ty).
+
+Inductive WfCtx : Ctx -> Prop :=
+| WfCtx_nil  :
+  WfCtx []
+| WfCtx_cons :
+    forall (Γ : Ctx) (x : Atom) (A : Ty),
+      WfCtx Γ -> x # map fst Γ -> WfCtx ((x, A) :: Γ).
+
+#[export] Hint Constructors WfCtx : core.
+
+Lemma WfCtx_app_cons :
+  forall (Γ1 Γ2 : Ctx) (x : Atom) (A : Ty),
+    WfCtx (Γ2 ++ (x, A) :: Γ1) -> WfCtx (Γ2 ++ Γ1).
+Proof.
+  induction Γ2 as [| [y B] Γ2' IH]; cbn; inversion 1; [easy |].
+  constructor.
+  - now apply IH in H2.
+  - unfold Fresh in *; rewrite map_app, !in_app_iff in *; cbn in *.
+    now firstorder.
+Qed.
+
+Definition Binds (Γ : Ctx) (x : Atom) (A : Ty) : Prop :=
+  In (x, A) Γ.
+
+Inductive Typing : Ctx -> Tm -> Ty -> Prop :=
+| Typing_fvar :
+  forall (Γ : Ctx) (x : Atom) (A : Ty),
+    WfCtx Γ ->
+    Binds Γ x A ->
+    Typing Γ x A
+| Typing_abs :
+  forall (Γ : Ctx) (t : Tm) (A B : Ty) (l : list Atom),
+    (forall x : Atom, x # l -> Typing ((x, A) :: Γ) (t {{ 0 ~> x }}) B) ->
+    Typing Γ (abs t) (TyFun A B)
+| Typing_app :
+  forall (Γ : Ctx) (t1 t2 : Tm) (A B : Ty),
+    Typing Γ t1 (TyFun A B) ->
+    Typing Γ t2 A ->
+    Typing Γ (app t1 t2) B.
+
+#[export] Hint Constructors Typing : Core.
+
+Lemma weakening_aux :
+  forall (Γ1 Γ2 Δ : Ctx) (t : Tm) (A : Ty),
+    Typing (Γ1 ++ Γ2) t A ->
+    WfCtx (Γ1 ++ Δ ++ Γ2) ->
+    Typing (Γ1 ++ Δ ++ Γ2) t A.
+Proof.
+  intros * Ht.
+  remember (Γ1 ++ Γ2) as G.
+  revert Γ1 Γ2 Δ HeqG.
+  induction Ht; intros; subst.
+  - constructor; [easy |].
+    unfold Binds in *.
+    rewrite !in_app_iff; rewrite in_app_iff in H0.
+    now firstorder.
+  - apply Typing_abs with (l ++ map fst Γ1 ++ map fst Δ ++ map fst Γ2).
+    intros.
+    red in H2; rewrite !in_app_iff in H2.
+    rewrite app_comm_cons.
+    apply H0; [now firstorder | easy |].
+    cbn; constructor; [easy |].
+    red; rewrite !map_app, !in_app_iff.
+    now firstorder.
+  - apply Typing_app with A.
+    + now apply IHHt1.
+    + now apply IHHt2.
+Qed.
+
+Lemma weakening :
+  forall (Γ Δ : Ctx) (t : Tm) (A : Ty),
+    WfCtx (Δ ++ Γ) ->
+    Typing Γ t A ->
+    Typing (Δ ++ Γ) t A.
+Proof.
+  now intros; apply weakening_aux with (Γ1 := []); cbn.
+Qed.
+
+Lemma lc_Typing :
+  forall (Γ : Ctx) (t : Tm) (A : Ty),
+    Typing Γ t A -> lc t.
+Proof.
+  induction 1; only 1, 3: now constructor.
+  apply lc_abs with l.
+  intros x Hx.
+  now apply H0.
+Qed.
+
+Lemma Binds_inv :
+  forall (Γ : Ctx) (x : Atom) (A B : Ty),
+    WfCtx Γ -> Binds Γ x A -> Binds Γ x B -> A = B.
+Proof.
+  induction 1; cbn; [easy |].
+  intros [ [= -> ->] |].
+  - intros [ [= ->] |]; [easy |].
+    contradiction H0.
+    rewrite in_map_iff.
+    now exists (x, B).
+  - intros [ [= -> ->] |].
+    + contradiction H0.
+      rewrite in_map_iff.
+      now exists (x, A).
+    + now apply IHWfCtx.
+Qed.
+
+Lemma Binds_app_cons_inv :
+  forall (Γ Δ : Ctx) (x y : Atom) (A B : Ty),
+    Binds (Δ ++ (x, A) :: Γ) y B ->
+      (x = y /\ A = B)
+        \/
+      Binds (Δ ++ Γ) y B.
+Proof.
+  induction Δ; cbn.
+  - now firstorder congruence.
+  - inversion 1; subst; [now firstorder |].
+    apply IHΔ in H0.
+    now firstorder.
+Qed.
+
+Lemma Typing_subst_aux :
+  forall (Γ Δ : Ctx) (x : Atom) (t u : Tm) (A B : Ty),
+    Typing (Δ ++ (x, A) :: Γ) t B ->
+    Typing Γ u A ->
+    Typing (Δ ++ Γ) (t [[ x := u ]]) B.
+Proof.
+  intros * Ht Hu.
+  remember (Δ ++ (x, A) :: Γ) as G.
+  revert Δ x A Γ HeqG Hu.
+  induction Ht as [? y B Hwf HB | ? t' B1 B2 l Hcof IH | ? t1 t2 B1 B2 Ht1 IH1 Ht2 IH2];
+    cbn; intros; subst.
+  - apply WfCtx_app_cons in Hwf as Hwf'.
+    decide (x = y); subst.
+    + replace B with A.
+      * now apply weakening.
+      * symmetry.
+        eapply (Binds_inv _ _ _ _ Hwf HB).
+        red; rewrite in_app_iff; cbn.
+        now firstorder.
+    + apply Binds_app_cons_inv in HB as [ [-> ->] |]; [easy |].
+      now constructor.
+  - apply Typing_abs with (x :: l).
+    intros y Hy; cbn in Hy.
+    assert (x <> y /\ y # l) as [Hxy Hyl] by firstorder.
+    rewrite open_subst; [| now firstorder | now apply lc_Typing in Hu].
+    now eapply (IH y Hyl ((y, B1) :: Δ)).
+  - econstructor.
+    + now eapply IH1.
+    + now eapply IH2.
+Qed.
+
+Lemma Typing_subst :
+  forall (Γ : Ctx) (x : Atom) (t u : Tm) (A B : Ty),
+    Typing ((x, A) :: Γ) t B ->
+    Typing Γ u A ->
+    Typing Γ (t [[ x := u ]]) B.
+Proof.
+  now intros; eapply Typing_subst_aux with (Δ := []) (A := A).
+Qed.
+
+Inductive Value : Tm -> Prop :=
+| Value_abs : forall t : Tm, lc (abs t) -> Value (abs t).
+
+#[export] Hint Constructors Value : core.
+
+Inductive Step : Tm -> Tm -> Prop :=
+| Step_FunComp :
+  forall (t1 t2 : Tm),
+    lc (abs t1) ->
+    Value t2 ->
+    Step (app (abs t1) t2) (t1 {{ 0 ~> t2 }})
+| Step_FunCongrL :
+  forall (t1 t1' t2 : Tm),
+    lc t2 ->
+    Step t1 t1' ->
+    Step (app t1 t2) (app t1' t2)
+| Step_FunCongrR :
+  forall (t1 t2 t2' : Tm),
+    Value t1 ->
+    Step t2 t2' ->
+    Step (app t1 t2) (app t1 t2').
+
+#[export] Hint Constructors Step : core.
+
+Lemma preservation :
+  forall (Γ : Ctx) (t1 t2 : Tm) (A : Ty),
+    Step t1 t2 ->
+    Typing Γ t1 A ->
+    Typing Γ t2 A.
+Proof.
+  intros * Hs Ht; revert t2 Hs.
+  induction Ht; intros; inversion Hs; subst.
+  - inversion Ht1; subst.
+    rewrite open_from_subst with (x := fresh (l ++ fv t3)) by solve_fresh.
+    apply Typing_subst with A; [| easy].
+    apply H4.
+    now solve_fresh.
+  - now econstructor; eauto.
+  - now econstructor; eauto.
+Qed.
+
+Lemma progress :
+  forall (t : Tm) (A : Ty),
+    Typing [] t A ->
+      Value t \/ exists t' : Tm, Step t t'.
+Proof.
+  intros t A Ht.
+  remember [] as Γ.
+  induction Ht; subst.
+  - now inversion H0.
+  - left; constructor.
+    apply lc_abs with l.
+    intros x Hx.
+    now eapply lc_Typing, H.
+  - destruct (IHHt1 eq_refl) as [ [t1' Hlc1] | [t1' Hs1] ].
+    + now destruct (IHHt2 eq_refl) as [ [t2' Hlc2] | [t2' Hs2] ]; eauto.
+    + now apply lc_Typing in Ht2; eauto.
+Qed.
+
+Lemma lc_open :
+  forall (t u : Tm),
+    lc (abs t) -> lc u ->
+      lc (t {{ 0 ~> u }}).
+Proof.
+  inversion 1; intros Hu.
+  rewrite (open_from_subst _ _ (fresh (l ++ fv t))) by solve_fresh.
+  apply lc_subst; [| easy].
+  apply Hcof.
+  now solve_fresh.
+Qed.
+
+Lemma lc_Value :
+  forall t : Tm,
+    Value t -> lc t.
+Proof.
+  now inversion 1.
+Qed.
+
+Lemma lc_Step_l :
+  forall t t' : Tm,
+    Step t t' -> lc t.
+Proof.
+  induction 1.
+  - constructor; [easy |].
+    now apply lc_Value.
+  - now constructor.
+  - constructor; [| easy ].
+    now apply lc_Value.
+Qed.
+
+Lemma lc_Step_r :
+  forall t t' : Tm,
+    Step t t' -> lc t'.
+Proof.
+  induction 1.
+  - apply lc_open; [easy |].
+    now apply lc_Value.
+  - now constructor.
+  - constructor; [| easy ].
+    now apply lc_Value.
+Qed.
+
+Lemma WfCtx_Typing :
+  forall (Γ : Ctx) (t : Tm) (A : Ty),
+    Typing Γ t A -> WfCtx Γ.
+Proof.
+  induction 1; [easy | | easy].
+  specialize (H0 (fresh l) (fresh_spec l)).
+  now inversion H0.
+Qed.
+
+Inductive Infer : Ctx -> Tm -> Ty -> Prop :=
+| Infer_fvar :
+  forall (Γ : Ctx) (x : Atom) (A : Ty),
+    Binds Γ x A -> Infer Γ x A
+| Infer_app  :
+  forall (Γ : Ctx) (t1 t2 : Tm) (A B : Ty),
+    Infer Γ t1 (TyFun A B) ->
+    Check Γ t2 A ->
+    Infer Γ (app t1 t2) B
+
+with Check : Ctx -> Tm -> Ty -> Prop :=
+| Check_Infer :
+  forall (Γ : Ctx) (t : Tm) (A : Ty),
+    Infer Γ t A ->
+    Check Γ t A
+| Check_abs :
+  forall (Γ : Ctx) (t : Tm) (A B : Ty) (l : list Atom)
+    (Hcof : forall x : Atom, x # l -> Check ((x, A) :: Γ) (t {{0 ~> x}}) B),
+    Check Γ (abs t) (TyFun A B).
+
+#[export] Hint Constructors Infer Check : core.
+
+Lemma Typing_Infer :
+  forall (Γ : Ctx) (t : Tm) (A : Ty),
+    WfCtx Γ -> Infer Γ t A -> Typing Γ t A
+
+with Typing_Check :
+  forall (Γ : Ctx) (t : Tm) (A : Ty),
+    WfCtx Γ -> Check Γ t A -> Typing Γ t A.
+Proof.
+  - intros Γ t A Hwf; destruct 1 as [Γ x A HB | Γ t1 t2 A B HI1 HC2].
+    + now constructor.
+    + apply Typing_app with A.
+      * now apply Typing_Infer.
+      * now apply Typing_Check.
+  - intros Γ t A Hwf; destruct 1 as [Γ t A Hi | Γ t A B l Hcof].
+    + now apply Typing_Infer.
+    + apply Typing_abs with (l ++ map fst Γ); intros x Hx.
+      red in Hx; rewrite in_app_iff in Hx.
+      apply Typing_Check.
+      * now firstorder.
+      * now apply Hcof; firstorder.
+Qed.
+
+Inductive Contraction : Tm -> Tm -> Prop :=
+| Contraction_Fun :
+  forall (t1 t2 : Tm),
+    lc (abs t1) ->
+    Value t2 ->
+    Contraction (app (abs t1) t2) (t1 {{ 0 ~> t2 }}).
+
+Inductive EvalCtx : Type :=
+| Hole : EvalCtx
+| FunCongrL :
+  forall (E : EvalCtx) (t2 : Tm) (Hlc2 : lc t2), EvalCtx
+| FunCongrR :
+  forall (t1 : Tm) (v1 : Value t1) (E : EvalCtx), EvalCtx.
+
+Fixpoint plug (E : EvalCtx) (t : Tm) : Tm :=
+match E with
+| Hole => t
+| FunCongrL E' t2 _ => app (plug E' t) t2
+| FunCongrR t1 _ E' => app t1 (plug E' t)
+end.
+
+Module inductive.
+
+Inductive Step' : Tm -> Tm -> Prop :=
+| mkStep' :
+  forall (E : EvalCtx) (t t' : Tm),
+    Contraction t t' -> Step' (plug E t) (plug E t').
+
+Hint Constructors Step' : core.
+
+Lemma Step'_spec :
+  forall t t' : Tm,
+    Step' t t' <-> Step t t'.
+Proof.
+  split.
+  - destruct 1 as [E t t' [] ].
+    induction E; cbn; intros.
+    + now constructor.
+    + now constructor; [| apply IHE].
+    + now constructor; [| apply IHE].
+  - induction 1.
+    + now apply (mkStep' Hole _ (t1 {{ 0 ~> t2 }})).
+    + destruct IHStep as [E u u' HC].
+      now apply (mkStep' (FunCongrL E t2 H)).
+    + destruct IHStep as [E u u' HC].
+      now apply (mkStep' (FunCongrR t1 H E)).
+Qed.
+
+End inductive.
+
+Module ex.
+
+Definition Step' (t t' : Tm) : Prop :=
+  exists (E : EvalCtx) (u u' : Tm),
+    t = plug E u /\
+    t' = plug E u' /\
+    Contraction u u'.
+
+Lemma Step'_spec :
+  forall t t' : Tm,
+    Step' t t' <-> Step t t'.
+Proof.
+  split.
+  - intros (E & u & u' & -> & -> & []); clear u u'.
+    induction E; cbn; intros.
+    + now constructor.
+    + now constructor; [| apply IHE].
+    + now constructor; [| apply IHE].
+  - induction 1.
+    + exists Hole.
+      now do 2 eexists.
+    + destruct IHStep as (E & u & u' & -> & -> & HC).
+      exists (FunCongrL E t2 H).
+      now do 2 eexists.
+    + destruct IHStep as (E & u & u' & -> & -> & HC).
+      exists (FunCongrR t1 H E).
+      now do 2 eexists.
+Qed.
+
+Lemma preservation_Contraction :
+  forall (Γ : Ctx) (t t' : Tm) (A : Ty),
+    Contraction t t' ->
+    Typing Γ t A ->
+    Typing Γ t' A.
+Proof.
+  induction 1; inversion 1; subst.
+  inversion H5; subst.
+  rewrite open_from_subst with (x := fresh (l ++ fv t1)) by solve_fresh.
+  apply Typing_subst with A0; [| easy].
+  apply H6.
+  now solve_fresh.
+Qed.
+
+Lemma preservation :
+  forall (Γ : Ctx) (t t' : Tm) (A : Ty),
+    Step' t t' ->
+    Typing Γ t A ->
+    Typing Γ t' A.
+Proof.
+  intros * (E & u & u' & -> & -> & HC).
+  revert A.
+  induction E; cbn; intros.
+  - now eapply preservation_Contraction; eauto.
+  - now inversion H; subst; econstructor; eauto.
+  - now inversion H; subst; econstructor; eauto.
+Qed.
+
+End ex.
+
+Module record.
+
+Record Step' (t t' : Tm) : Prop := mkStep'
+{
+  E : EvalCtx;
+  u : Tm;
+  u' : Tm;
+  Ht : t = plug E u;
+  Ht' : t' = plug E u';
+  HC : Contraction u u';
+}.
+
+Lemma Step'_spec :
+  forall t t' : Tm,
+    Step' t t' <-> Step t t'.
+Proof.
+  split.
+  - intros [E u u' -> -> [] ].
+    induction E; cbn; intros.
+    + now constructor.
+    + now constructor; [| apply IHE].
+    + now constructor; [| apply IHE].
+  - induction 1.
+    + now eapply (mkStep' _ _ Hole).
+    + destruct IHStep as [E u u' -> -> HC].
+      now eapply (mkStep' _ _ (FunCongrL E t2 H)).
+    + destruct IHStep as [E u u' -> -> HC].
+      now eapply (mkStep' _ _ (FunCongrR t1 H E)).
+Qed.
+
+End record.
